\section{Welford Algorithm for Calculating Variance}

We want to calculate the mean and unbiased variance of a numeric list $X=[x_1 \ldots x_{N}]$ that has a length $N$:

\begin{align*}
\mu_{N} &= \frac{1}{N}\sum^{N}_{i=1} x_i \\
\sigma^2_{N} &=\frac{1}{N-1} \sum^{N}_{i-1}\left(x_i - \mu_{N}\right)^2 
\end{align*}

The two computations mentioned above scan the input list elements twice, each with a complexity of $O(N)$. Now, suppose we add a new element $x_{N}$ to the list and want to update the mean $\mu_{N+1}$ and variance $\sigma_{N+1}$. Instead of repeating the two $O(N)$ computations, can we update $\mu_{N+1}$ and $\sigma_{N+1}^2$ using the existing values of $N$, $\mu_{N}$, and $\sigma_{N}^2$? If so, we can compute $\mu_N$ and $\sigma_{N}^2$ for the entire list portion by portion for extremely long lists.

Let's start from the new mean $\mu_{N+1}$ from $x_{N+1}$ and $\mu_{N}$. This is rather straightforward:

\begin{align}
\mu_{N+1} &= \frac{x_{N+1}+N\mu_{N}}{N+1} \nonumber \\
&=\mu_{N}+\frac{x_{N+1}-\mu_{N}}{N+1}\tag{1}\label{eq:1}
\end{align}

Subsitute $N+1$ with $N$ in equation \eqref{eq:1}, we can also get:

\begin{equation}
\mu_{N}=\mu_{N-1}+\frac{x_{N}-\mu_{N-1}}{N}\tag{2}\label{eq:2}
\end{equation}


Let's define a quantity called $s_N$:

\begin{align*}
s_{N} &= \sum^{N}_{i=1}(x_i - \mu_{N})^2 \\
&=\sum^{N-1}_{i=1}\left(x_i-\mu_{N}\right)^2+\left(x_N-\mu_{N}\right)^2 \tag{3}\label{eq:3}
\end{align*}

Substitue equation \eqref{eq:2} into equation \eqref{eq:3}:

\begin{align*}
s_N &= \sum_{i=1}^{N-1}\left(x_i-\mu_{N-1}-\frac{x_N-\mu_{N-1}}{N} \right)^2 + \left(x_N-\mu_{N-1}-\frac{x_N-\mu_{N-1}}{N}\right)^2 \\
&=\sum_{i=1}^{N-1}\left(\left(x_i-\mu_{N-1}\right)-\frac{1}{N}\left(x_N-\mu_{N-1}\right)\right)^2+\left(\frac{N-1}{N}(x_N-\mu_{N-1})\right)^2 \tag{4}\label{eq:4}
\end{align*}

Let's first look into the first component of equation \eqref{eq:4}:

\begin{align*}
&\sum_{i=1}^{N-1}\left(\left(x_i-\mu_{N-1}\right)-\frac{1}{N}\left(x_N-\mu_{N-1}\right)\right)^2 \\
=&\sum_{i=1}^{N-1}\left((x_i-\mu_{N-1})^2-\textcolor{red}{\frac{2}{N}(x_i-\mu_{N-1})(x_N-\mu_{N-1})}+(x_N-\mu_{N-1})^2\right) 
\end{align*}

The equation in red is actually equal to zero.

\begin{align*}
&\sum_{i=1}^{N-1}\frac{2}{N}(x_i-\mu_{N-1})(x_N-\mu_{N-1}) \\
=&\frac{2}{N}(N-1)(x_N-\mu_{N-1})\left(\sum_{i=0}^{N-1}x_i-(N-1)\mu_{N-1}\right) \\
=&\frac{2}{N}(N-1)(x_N-\mu_{N-1})\left(\sum_{i=0}^{N-1}x_i-\sum_{i=0}^{N-1}x_i\right) \\
=&\ 0
\end{align*}

Substitue these results into equation \eqref{eq:4}:

\begin{align*}
s_{N} &=\sum_{i=1}^{N-1}\left((x_i-\mu_{N-1})^2+\frac{1}{N}(x_N-\mu_{N-1})^2\right) + \left(\frac{N-1}{N}(x_N-\mu_{N-1})\right)^2 \\
&=\frac{N-1}{N^2}(x_N-\mu_{N-1})^2+\frac{(N-1)^2}{N^2}(x_N-\mu_{N-1})^2+\sum_{i=1}^{N-1}(x_i-\mu_{N-1})^2 \\
&=\left[\frac{N-1}{N^2} + \frac{(N-1)^2}{N^2}\right](x_N-\mu_{N-1})^2+\sum_{i=1}^{N-1}\left(x_i-\mu_{N-1}^2\right) \\
s_N&=s_{N-1} + \frac{N-1}{N}(x_N-\mu_{N-1})^2 \tag{5}\label{eq:5}
\end{align*}

We can manipulate equation \eqref{eq:5} further by given:
\begin{align*}
(N-1)\mu_{N-1} &= N\mu_N-x_N \\
\mu_{N-1} &= \frac{N\mu_{N}-x_N}{N-1}
\end{align*}

substitute it into equation \eqref{eq:5}:

\begin{align*}
s_N&=s_{N-1} + (x_N-\mu_{N-1})\frac{N-1}{N}(x_N-\frac{N\mu_{N}-x_N}{N-1}) \\
s_N&=s_{N-1} + (x_N-\mu_{N-1})(x_N-\mu_{N})
\end{align*}

Suppose we use Welford's algorithm to calculate the mean and variance for lists $A$ and $B$.
Now we want to obtain the mean and variance for $AB$, which is the concatenation of $A$ and $B$. To do this, we can use the formula described in \cite{chan1982updating}.

\begin{align*}
N_{AB} &= N_{A} + N_{B} \\
\delta &= \mu_B - \mu_A \\
\mu_{AB} &= \mu_A+\delta\frac{N_B}{N_{AB}} \\
M_{2, AB} &=M_{2,A}+M_{2,B}+\delta^2*\frac{N_A N_B}{N_{AB}}
\end{align*}